Validator/Expr/IfExpr.lean
@@ -10,22 +10,22 @@ abbrev IfExprs n φ l := Vec (IfExpr n φ) l
 namespace IfExpr
 
 def eval {α: Type}
-  (g: Grammar n φ) (Φ: φ -> α -> Prop) [DecidableRel Φ]
+  (G: Grammar n φ) (Φ: φ -> α -> Prop) [DecidableRel Φ]
   (ifExpr: IfExpr n φ) (t: α): Rule n φ :=
   match ifExpr with
   | (cnd, thn) =>
     if Φ cnd t
-    then g.lookup thn
+    then G.lookup thn
     else Regex.emptyset
 
 def evals {α: Type} {n: Nat}
-  (g: Grammar n φ) (Φ: φ -> α -> Prop) [DecidableRel Φ]
+  (G: Grammar n φ) (Φ: φ -> α -> Prop) [DecidableRel Φ]
   (ifExprs: IfExprs n φ l) (t: α): Rules n φ l :=
-  Vec.map ifExprs (fun x => eval g Φ x t)
+  Vec.map ifExprs (fun x => eval G Φ x t)
 
 theorem evals_nil_is_nil {α: Type} {n: Nat}
-  (g: Grammar n φ) (Φ: φ -> α -> Prop) [DecidableRel Φ]
+  (G: Grammar n φ) (Φ: φ -> α -> Prop) [DecidableRel Φ]
   (a: α):
-  evals g Φ (n := n) Vec.nil a = Vec.nil := by
+  evals G Φ (n := n) Vec.nil a = Vec.nil := by
   unfold evals
   simp only [Vec.map_nil]
