Validator/Learning/Compress.lean
@@ -21,7 +21,7 @@ namespace Compress
 
 -- deriv is the same as Basic's deriv function, except that it includes the use of the compress and expand functions.
 def derive [DecidableEq φ]
-  (g: Grammar n φ) (Φ : φ → α → Prop) [DecidableRel Φ]
+  (G: Grammar n φ) (Φ : φ → α → Prop) [DecidableRel Φ]
   (xs: Rules n φ l) (t: Hedge.Node α): Rules n φ l :=
   if List.all xs.toList Regex.unescapable
   then xs
@@ -29,29 +29,29 @@ def derive [DecidableEq φ]
     match t with
     | Hedge.Node.mk label children =>
       let ifexprs: IfExprs n φ (Symbol.nums xs) := Enter.deriveEnter xs
-      let childxs: Rules n φ (Symbol.nums xs) := IfExpr.evals g Φ ifexprs label
+      let childxs: Rules n φ (Symbol.nums xs) := IfExpr.evals G Φ ifexprs label
       -- cchildxs = compressed expressions to evaluate on children.
       let ⟨n, cchildxs, indices⟩ := Compress.compress childxs
       -- cdchildxs = compressed derivatives of children.
-      let cdchildxs := List.foldl (derive g Φ) cchildxs children
+      let cdchildxs := List.foldl (derive G Φ) cchildxs children
       -- dchildxs = uncompressed derivatives of children.
       let dchildxs := Compress.expand indices cdchildxs
       Leave.deriveLeaves xs (Vec.map dchildxs Rule.nullable)
 
 def derivs [DecidableEq φ]
-  (g: Grammar n φ) (Φ : φ → α → Prop) [DecidableRel Φ]
+  (G: Grammar n φ) (Φ : φ → α → Prop) [DecidableRel Φ]
   (x: Rule n φ) (hedge: Hedge α): Rule n φ :=
-  let dxs := List.foldl (derive g Φ) (Vec.cons x Vec.nil) hedge
+  let dxs := List.foldl (derive G Φ) (Vec.cons x Vec.nil) hedge
   dxs.head
 
 def validate [DecidableEq φ]
-  (g: Grammar n φ) (Φ : φ → α → Prop) [DecidableRel Φ]
+  (G: Grammar n φ) (Φ : φ → α → Prop) [DecidableRel Φ]
   (x: Rule n φ) (hedge: Hedge α): Bool :=
-  let dx := derivs g Φ x hedge
+  let dx := derivs G Φ x hedge
   Rule.nullable dx
 
-def run [DecidableEq α] (g: Grammar n (Pred α)) (t: Hedge.Node α): Bool :=
-  validate g Pred.eval g.start [t]
+def run [DecidableEq α] (G: Grammar n (Pred α)) (t: Hedge.Node α): Bool :=
+  validate G Pred.eval G.start [t]
 
 -- Tests
 
