Validator/Learning/Memoize.lean
@@ -11,12 +11,12 @@ import Validator.Learning.Parser
 namespace Memoize
 
 def validate {m} [DecidableEq φ] [ValidateM m n φ α]
-  (g: Grammar n φ) (Φ : φ → α → Prop) [DecidableRel Φ]
+  (G: Grammar n φ) (Φ : φ → α → Prop) [DecidableRel Φ]
   (x: Rule n φ): m Bool :=
-  Parser.validate g Φ x
+  Parser.validate G Φ x
 
-def run [DecidableEq α] [Hashable α] (g: Grammar n (Pred α)) (t: Hedge.Node α): Except String Bool :=
-  TreeParserMemM.run' (n := n) (φ := Pred α) (validate g Pred.eval g.start) t
+def run [DecidableEq α] [Hashable α] (G: Grammar n (Pred α)) (t: Hedge.Node α): Except String Bool :=
+  TreeParserMemM.run' (n := n) (φ := Pred α) (validate G Pred.eval G.start) t
 
 -- Tests
 
